\begin{center}
	\begin{minipage}{0.3\linewidth}
		\begin{equation*}
		S_P = 
			\begin{bmatrix}
				-1 & 1 & 1 \\
				0 & 1 & 0
			\end{bmatrix}
		\end{equation*}
	\end{minipage}
	\begin{minipage}{0.6\linewidth}
		\begin{equation*}
		    V_P = \begin{Bmatrix}
		              \begin{bmatrix}
		                    -x' + y' + z' = 1 \\
		                    y' = y + 1
		               \end{bmatrix}, \\ \\
		               \begin{bmatrix}
		                     -x' + y' + z' = -x + y + z - 5 \\
		                    y' = y - 3y
		               \end{bmatrix}
		    \end{Bmatrix}
		\end{equation*}
	\end{minipage}
\end{center}
%\caption{\qvasr abstraction $A_p = (S, V)$ of $P$.}